pulse/share/steel/examples/pulse/dice/l0/L0Types.fst
@@ -1,5 +1,4 @@
 module L0Types
-open Pulse.Main
 open Pulse.Steel.Wrapper
 open Steel.ST.Util 
 open Steel.ST.Array
@@ -14,86 +13,14 @@ module U32 = FStar.UInt32
 open Array
 open HACL
 
-assume
-val x509_version_t : Type0
+let x509_version_t : Type0 = admit()
 
-assume
-val x509_serialNumber_t : Type0
+let x509_serialNumber_t : Type0 = admit()
 
-assume
-val deviceIDCRI_t : Type0
+let deviceIDCRI_t : Type0 = admit()
 
-assume
-val deviceIDCSR_t (len: US.t) : Type0
+let deviceIDCSR_t (len: US.t) : Type0 = admit()
 
-assume
-val aliasKeyTBS_t : Type0
+let aliasKeyTBS_t : Type0 = admit()
 
-assume
-val aliasKeyCRT_t (len: US.t) : Type0
-
-(* L0 Context *)
-noeq
-type l0_context = { cdi: A.larray U8.t (US.v dice_digest_len); }
-
-let l0_context_perm (c:l0_context) : vprop
-  = exists_ (fun (s:elseq U8.t dice_digest_len) -> A.pts_to c.cdi full_perm s) `star`
-    pure (A.is_full_array c.cdi)
-
-let mk_l0_context cdi : l0_context = {cdi}
-
-(* L0 Record *)
-noeq
-type deviceIDCSR_ingredients_t = {
-  ku        : U32.t;
-  version   : x509_version_t;
-  s_common  : string;
-  s_org     : string;
-  s_country : string;
-}
-
-noeq
-type aliasKeyCRT_ingredients_t = {
-  version       : x509_version_t;
-  serialNumber  : x509_serialNumber_t;
-  i_common      : string;
-  i_org         : string;
-  i_country     : string;
-  notBefore     : US.t; (* UTC_TIME *)
-  notAfter      : US.t; (* Generalized_Time *)
-  s_common      : string;
-  s_org         : string;
-  s_country     : string;
-  ku            : U32.t;
-  l0_version    : U32.t;
-}
-
-noeq
-type l0_record_t = {
-  fwid: A.larray U8.t (US.v v32us);
-  deviceID_label_len: hkdf_lbl_len;
-  deviceID_label: A.larray U8.t (US.v deviceID_label_len); (* public bytes *)
-  aliasKey_label_len: hkdf_lbl_len;
-  aliasKey_label: A.larray U8.t (US.v aliasKey_label_len); (* public bytes *)
-  deviceIDCSR_ingredients: deviceIDCSR_ingredients_t;
-  aliasKeyCRT_ingredients: aliasKeyCRT_ingredients_t;
-}
-
-noeq
-type l0_record_repr = {
-  fwid: Seq.seq U8.t;
-  deviceID_label: Seq.seq U8.t;
-  aliasKey_label: Seq.seq U8.t;
-}
-
-let mk_l0_repr fwid deviceID_label aliasKey_label 
-  = {fwid; deviceID_label; aliasKey_label}
-
-let l0_record_perm (record:l0_record_t) (repr:l0_record_repr) : vprop =
-  A.pts_to record.fwid full_perm repr.fwid `star`
-  A.pts_to record.deviceID_label full_perm repr.deviceID_label `star`
-  A.pts_to record.aliasKey_label full_perm repr.aliasKey_label `star`
-  pure (
-    valid_hkdf_lbl_len record.deviceID_label_len /\
-    valid_hkdf_lbl_len record.aliasKey_label_len
-  )
+let aliasKeyCRT_t (len: US.t) : Type0 = admit()
