pulse/share/steel/examples/pulse/dice/l0/L0Types.fsti
@@ -1,0 +1,90 @@
+module L0Types
+open Pulse.Steel.Wrapper
+open Steel.ST.Util 
+open Steel.ST.Array
+open Steel.FractionalPermission
+open FStar.Ghost
+module R = Steel.ST.Reference
+module A = Steel.ST.Array
+module T = FStar.Tactics
+module US = FStar.SizeT
+module U8 = FStar.UInt8
+module U32 = FStar.UInt32
+open Array
+open HACL
+
+val x509_version_t : Type0
+
+val x509_serialNumber_t : Type0
+
+val deviceIDCRI_t : Type0
+
+val deviceIDCSR_t (len: US.t) : Type0
+
+val aliasKeyTBS_t : Type0
+
+val aliasKeyCRT_t (len: US.t) : Type0
+
+noeq
+type l0_context = { cdi: A.larray U8.t (US.v dice_digest_len); }
+
+let l0_context_perm (c:l0_context) : vprop
+  = exists_ (fun (s:elseq U8.t dice_digest_len) -> A.pts_to c.cdi full_perm s) `star`
+    pure (A.is_full_array c.cdi)
+
+let mk_l0_context cdi : l0_context = {cdi}
+
+noeq
+type deviceIDCSR_ingredients_t = {
+  ku        : U32.t;
+  version   : x509_version_t;
+  s_common  : string;
+  s_org     : string;
+  s_country : string;
+}
+
+noeq
+type aliasKeyCRT_ingredients_t = {
+  version       : x509_version_t;
+  serialNumber  : x509_serialNumber_t;
+  i_common      : string;
+  i_org         : string;
+  i_country     : string;
+  notBefore     : US.t; (* UTC_TIME *)
+  notAfter      : US.t; (* Generalized_Time *)
+  s_common      : string;
+  s_org         : string;
+  s_country     : string;
+  ku            : U32.t;
+  l0_version    : U32.t;
+}
+
+noeq
+type l0_record_t = {
+  fwid: A.larray U8.t (US.v v32us);
+  deviceID_label_len: hkdf_lbl_len;
+  deviceID_label: A.larray U8.t (US.v deviceID_label_len); (* public bytes *)
+  aliasKey_label_len: hkdf_lbl_len;
+  aliasKey_label: A.larray U8.t (US.v aliasKey_label_len); (* public bytes *)
+  deviceIDCSR_ingredients: deviceIDCSR_ingredients_t;
+  aliasKeyCRT_ingredients: aliasKeyCRT_ingredients_t;
+}
+
+noeq
+type l0_record_repr = {
+  fwid: Seq.seq U8.t;
+  deviceID_label: Seq.seq U8.t;
+  aliasKey_label: Seq.seq U8.t;
+}
+
+let mk_l0_repr fwid deviceID_label aliasKey_label
+  = {fwid; deviceID_label; aliasKey_label}
+
+let l0_record_perm (record:l0_record_t) (repr:l0_record_repr) : vprop =
+  A.pts_to record.fwid full_perm repr.fwid `star`
+  A.pts_to record.deviceID_label full_perm repr.deviceID_label `star`
+  A.pts_to record.aliasKey_label full_perm repr.aliasKey_label `star`
+  pure (
+    valid_hkdf_lbl_len record.deviceID_label_len /\
+    valid_hkdf_lbl_len record.aliasKey_label_len
+  )
