pulse/share/steel/examples/pulse/lib/PulseHashTable.fst
@@ -16,58 +16,6 @@ open Pulse.Class.BoundedIntegers
 
 #push-options "--using_facts_from '* -FStar.Tactics -FStar.Reflection'"
 
-type pos_us = n:US.t{US.v n > 0}
-
-noeq
-type pht_sig_us = {
-  keyt : eqtype;
-  valt : Type0;
-  hashf : keyt -> US.t;
-}
-let mk_pht_sig_us keyt valt hashf : pht_sig_us = { keyt; valt; hashf }
-
-noeq
-type ht_t (s : pht_sig_us) = {
-  sz : pos_us;
-  contents : A.larray (cell s.keyt s.valt) (US.v sz);
-}
-let mk_ht (#s:pht_sig_us) (sz:pos_us) 
-          (contents:A.larray (cell s.keyt s.valt) (US.v sz))
-  : ht_t s 
-  = { sz; contents; }
-
-let s_to_ps (s:pht_sig_us) : pht_sig
-  = { keyt = s.keyt; valt = s.valt; hashf = (fun k -> US.v (s.hashf k)) }
-
-let mk_init_pht (#s:pht_sig_us) (sz:pos_us)
-  : pht_t (s_to_ps s)
-  = 
-  { sz = US.v sz;
-    spec = (fun (k:s.keyt) -> None);
-    repr = Seq.create (US.v sz) Clean;
-    inv = (); }
-
-let models (s:pht_sig_us) (ht:ht_t s) (pht:pht_t (s_to_ps s)) : vprop
-= A.pts_to ht.contents full_perm pht.repr `star`
-  pure (
-    US.v ht.sz == pht.sz /\
-    A.is_full_array ht.contents
-  )
-
-let ht_perm (s:pht_sig_us) (ht: ht_t s) : vprop
-  = exists_ (fun (pht:pht_t (s_to_ps s)) -> models s ht pht) // FIXME: this is erasing the pht
-
-type locked_ht_t (s:pht_sig_us) = ht:ht_t s & LK.lock (ht_perm s ht)
-
-let canonical_index_us (#s:pht_sig_us) (k:s.keyt) (sz:pos_us) 
-  : US.t = s.hashf k % sz
-
-let modulo_us (v1 v2:US.t) (m:pos_us) (_:squash(US.fits (US.v v1 + US.v v2)))
-  : US.t 
-  = (v1 + v2) % m
-
-let pht_sz #s (pht:pht_t s) : pos = pht.sz
-
 ```pulse
 fn pulse_lookup_index (#s:pht_sig_us)
                       (#pht:erased (pht_t (s_to_ps s)))
@@ -138,7 +86,7 @@ fn pulse_lookup_index (#s:pht_sig_us)
 ```
 
 ```pulse
-fn lookup (#s:pht_sig_us)
+fn _lookup (#s:pht_sig_us)
           (#pht:erased (pht_t (s_to_ps s)))
           (ht:ht_t s) (k:s.keyt)
   requires models s ht pht
@@ -152,9 +100,10 @@ fn lookup (#s:pht_sig_us)
   }
 }
 ```
+let lookup #s #pht ht k = _lookup #s #pht ht k
 
 ```pulse
-fn insert (#s:pht_sig_us)
+fn _insert (#s:pht_sig_us)
           (#pht:(p:erased (pht_t (s_to_ps s)){PHT.not_full p.repr}))
           (ht:ht_t s) (k:s.keyt) (v:s.valt)
   requires models s ht pht
@@ -232,9 +181,10 @@ fn insert (#s:pht_sig_us)
   fold (models s ht (PHT.insert pht k v));
 }
 ```
+let insert #s #pht ht k v = _insert #s #pht ht k v
 
 ```pulse
-fn delete (#s:pht_sig_us)
+fn _delete (#s:pht_sig_us)
           (#pht:erased (pht_t (s_to_ps s)))
           (ht:ht_t s) (k:s.keyt)
   requires models s ht pht
@@ -294,9 +244,10 @@ fn delete (#s:pht_sig_us)
   fold (models s ht (PHT.delete pht k));
 }
 ```
+let delete #s #pht ht k = _delete #s #pht ht k
 
 ```pulse
-fn not_full (#s:pht_sig_us) (#pht:erased (pht_t (s_to_ps s))) (ht:ht_t s)
+fn _not_full (#s:pht_sig_us) (#pht:erased (pht_t (s_to_ps s))) (ht:ht_t s)
   requires models s ht pht
   returns b:bool
   ensures models s ht pht ** 
@@ -330,3 +281,4 @@ fn not_full (#s:pht_sig_us) (#pht:erased (pht_t (s_to_ps s))) (ht:ht_t s)
   res
 }
 ```
+let not_full #s #pht ht = _not_full #s #pht ht
